Add codomain to lambda and complete validity

theories/autosubst/AST.v
@@ -9,7 +9,7 @@ Inductive term : Type :=
   | var : nat -> term
   | Sort : mode -> level -> term
   | Pi : level -> level -> mode -> mode -> term -> term -> term
-  | lam : mode -> term -> term -> term
+  | lam : mode -> term -> term -> term -> term
   | app : term -> term -> term
   | Erased : term -> term
   | erase : term -> term
@@ -46,13 +46,16 @@ exact (eq_trans
          (ap (fun x => Pi t0 t1 t2 t3 t4 x) H5)).
 Qed.
 
-Lemma congr_lam {s0 : mode} {s1 : term} {s2 : term} {t0 : mode} {t1 : term}
-  {t2 : term} (H0 : s0 = t0) (H1 : s1 = t1) (H2 : s2 = t2) :
-  lam s0 s1 s2 = lam t0 t1 t2.
+Lemma congr_lam {s0 : mode} {s1 : term} {s2 : term} {s3 : term} {t0 : mode}
+  {t1 : term} {t2 : term} {t3 : term} (H0 : s0 = t0) (H1 : s1 = t1)
+  (H2 : s2 = t2) (H3 : s3 = t3) : lam s0 s1 s2 s3 = lam t0 t1 t2 t3.
 Proof.
 exact (eq_trans
-         (eq_trans (eq_trans eq_refl (ap (fun x => lam x s1 s2) H0))
-            (ap (fun x => lam t0 x s2) H1)) (ap (fun x => lam t0 t1 x) H2)).
+         (eq_trans
+            (eq_trans (eq_trans eq_refl (ap (fun x => lam x s1 s2 s3) H0))
+               (ap (fun x => lam t0 x s2 s3) H1))
+            (ap (fun x => lam t0 t1 x s3) H2))
+         (ap (fun x => lam t0 t1 t2 x) H3)).
 Qed.
 
 Lemma congr_app {s0 : term} {s1 : term} {t0 : term} {t1 : term}
@@ -144,8 +147,9 @@ Fixpoint ren_term (xi_term : nat -> nat) (s : term) {struct s} : term :=
   | Pi s0 s1 s2 s3 s4 s5 =>
       Pi s0 s1 s2 s3 (ren_term xi_term s4)
         (ren_term (upRen_term_term xi_term) s5)
-  | lam s0 s1 s2 =>
+  | lam s0 s1 s2 s3 =>
       lam s0 (ren_term xi_term s1) (ren_term (upRen_term_term xi_term) s2)
+        (ren_term (upRen_term_term xi_term) s3)
   | app s0 s1 => app (ren_term xi_term s0) (ren_term xi_term s1)
   | Erased s0 => Erased (ren_term xi_term s0)
   | erase s0 => erase (ren_term xi_term s0)
@@ -177,9 +181,10 @@ term :=
   | Pi s0 s1 s2 s3 s4 s5 =>
       Pi s0 s1 s2 s3 (subst_term sigma_term s4)
         (subst_term (up_term_term sigma_term) s5)
-  | lam s0 s1 s2 =>
+  | lam s0 s1 s2 s3 =>
       lam s0 (subst_term sigma_term s1)
         (subst_term (up_term_term sigma_term) s2)
+        (subst_term (up_term_term sigma_term) s3)
   | app s0 s1 => app (subst_term sigma_term s0) (subst_term sigma_term s1)
   | Erased s0 => Erased (subst_term sigma_term s0)
   | erase s0 => erase (subst_term sigma_term s0)
@@ -221,9 +226,10 @@ subst_term sigma_term s = s :=
       congr_Pi (eq_refl s0) (eq_refl s1) (eq_refl s2) (eq_refl s3)
         (idSubst_term sigma_term Eq_term s4)
         (idSubst_term (up_term_term sigma_term) (upId_term_term _ Eq_term) s5)
-  | lam s0 s1 s2 =>
+  | lam s0 s1 s2 s3 =>
       congr_lam (eq_refl s0) (idSubst_term sigma_term Eq_term s1)
         (idSubst_term (up_term_term sigma_term) (upId_term_term _ Eq_term) s2)
+        (idSubst_term (up_term_term sigma_term) (upId_term_term _ Eq_term) s3)
   | app s0 s1 =>
       congr_app (idSubst_term sigma_term Eq_term s0)
         (idSubst_term sigma_term Eq_term s1)
@@ -274,10 +280,12 @@ ren_term xi_term s = ren_term zeta_term s :=
         (extRen_term xi_term zeta_term Eq_term s4)
         (extRen_term (upRen_term_term xi_term) (upRen_term_term zeta_term)
            (upExtRen_term_term _ _ Eq_term) s5)
-  | lam s0 s1 s2 =>
+  | lam s0 s1 s2 s3 =>
       congr_lam (eq_refl s0) (extRen_term xi_term zeta_term Eq_term s1)
         (extRen_term (upRen_term_term xi_term) (upRen_term_term zeta_term)
            (upExtRen_term_term _ _ Eq_term) s2)
+        (extRen_term (upRen_term_term xi_term) (upRen_term_term zeta_term)
+           (upExtRen_term_term _ _ Eq_term) s3)
   | app s0 s1 =>
       congr_app (extRen_term xi_term zeta_term Eq_term s0)
         (extRen_term xi_term zeta_term Eq_term s1)
@@ -329,10 +337,12 @@ subst_term sigma_term s = subst_term tau_term s :=
         (ext_term sigma_term tau_term Eq_term s4)
         (ext_term (up_term_term sigma_term) (up_term_term tau_term)
            (upExt_term_term _ _ Eq_term) s5)
-  | lam s0 s1 s2 =>
+  | lam s0 s1 s2 s3 =>
       congr_lam (eq_refl s0) (ext_term sigma_term tau_term Eq_term s1)
         (ext_term (up_term_term sigma_term) (up_term_term tau_term)
            (upExt_term_term _ _ Eq_term) s2)
+        (ext_term (up_term_term sigma_term) (up_term_term tau_term)
+           (upExt_term_term _ _ Eq_term) s3)
   | app s0 s1 =>
       congr_app (ext_term sigma_term tau_term Eq_term s0)
         (ext_term sigma_term tau_term Eq_term s1)
@@ -384,12 +394,15 @@ Fixpoint compRenRen_term (xi_term : nat -> nat) (zeta_term : nat -> nat)
         (compRenRen_term (upRen_term_term xi_term)
            (upRen_term_term zeta_term) (upRen_term_term rho_term)
            (up_ren_ren _ _ _ Eq_term) s5)
-  | lam s0 s1 s2 =>
+  | lam s0 s1 s2 s3 =>
       congr_lam (eq_refl s0)
         (compRenRen_term xi_term zeta_term rho_term Eq_term s1)
         (compRenRen_term (upRen_term_term xi_term)
            (upRen_term_term zeta_term) (upRen_term_term rho_term)
            (up_ren_ren _ _ _ Eq_term) s2)
+        (compRenRen_term (upRen_term_term xi_term)
+           (upRen_term_term zeta_term) (upRen_term_term rho_term)
+           (up_ren_ren _ _ _ Eq_term) s3)
   | app s0 s1 =>
       congr_app (compRenRen_term xi_term zeta_term rho_term Eq_term s0)
         (compRenRen_term xi_term zeta_term rho_term Eq_term s1)
@@ -448,12 +461,15 @@ subst_term tau_term (ren_term xi_term s) = subst_term theta_term s :=
         (compRenSubst_term (upRen_term_term xi_term) (up_term_term tau_term)
            (up_term_term theta_term) (up_ren_subst_term_term _ _ _ Eq_term)
            s5)
-  | lam s0 s1 s2 =>
+  | lam s0 s1 s2 s3 =>
       congr_lam (eq_refl s0)
         (compRenSubst_term xi_term tau_term theta_term Eq_term s1)
         (compRenSubst_term (upRen_term_term xi_term) (up_term_term tau_term)
            (up_term_term theta_term) (up_ren_subst_term_term _ _ _ Eq_term)
            s2)
+        (compRenSubst_term (upRen_term_term xi_term) (up_term_term tau_term)
+           (up_term_term theta_term) (up_ren_subst_term_term _ _ _ Eq_term)
+           s3)
   | app s0 s1 =>
       congr_app (compRenSubst_term xi_term tau_term theta_term Eq_term s0)
         (compRenSubst_term xi_term tau_term theta_term Eq_term s1)
@@ -523,12 +539,15 @@ ren_term zeta_term (subst_term sigma_term s) = subst_term theta_term s :=
         (compSubstRen_term (up_term_term sigma_term)
            (upRen_term_term zeta_term) (up_term_term theta_term)
            (up_subst_ren_term_term _ _ _ Eq_term) s5)
-  | lam s0 s1 s2 =>
+  | lam s0 s1 s2 s3 =>
       congr_lam (eq_refl s0)
         (compSubstRen_term sigma_term zeta_term theta_term Eq_term s1)
         (compSubstRen_term (up_term_term sigma_term)
            (upRen_term_term zeta_term) (up_term_term theta_term)
            (up_subst_ren_term_term _ _ _ Eq_term) s2)
+        (compSubstRen_term (up_term_term sigma_term)
+           (upRen_term_term zeta_term) (up_term_term theta_term)
+           (up_subst_ren_term_term _ _ _ Eq_term) s3)
   | app s0 s1 =>
       congr_app
         (compSubstRen_term sigma_term zeta_term theta_term Eq_term s0)
@@ -607,12 +626,15 @@ subst_term tau_term (subst_term sigma_term s) = subst_term theta_term s :=
         (compSubstSubst_term (up_term_term sigma_term)
            (up_term_term tau_term) (up_term_term theta_term)
            (up_subst_subst_term_term _ _ _ Eq_term) s5)
-  | lam s0 s1 s2 =>
+  | lam s0 s1 s2 s3 =>
       congr_lam (eq_refl s0)
         (compSubstSubst_term sigma_term tau_term theta_term Eq_term s1)
         (compSubstSubst_term (up_term_term sigma_term)
            (up_term_term tau_term) (up_term_term theta_term)
            (up_subst_subst_term_term _ _ _ Eq_term) s2)
+        (compSubstSubst_term (up_term_term sigma_term)
+           (up_term_term tau_term) (up_term_term theta_term)
+           (up_subst_subst_term_term _ _ _ Eq_term) s3)
   | app s0 s1 =>
       congr_app
         (compSubstSubst_term sigma_term tau_term theta_term Eq_term s0)
@@ -742,10 +764,12 @@ Fixpoint rinst_inst_term (xi_term : nat -> nat) (sigma_term : nat -> term)
         (rinst_inst_term xi_term sigma_term Eq_term s4)
         (rinst_inst_term (upRen_term_term xi_term) (up_term_term sigma_term)
            (rinstInst_up_term_term _ _ Eq_term) s5)
-  | lam s0 s1 s2 =>
+  | lam s0 s1 s2 s3 =>
       congr_lam (eq_refl s0) (rinst_inst_term xi_term sigma_term Eq_term s1)
         (rinst_inst_term (upRen_term_term xi_term) (up_term_term sigma_term)
            (rinstInst_up_term_term _ _ Eq_term) s2)
+        (rinst_inst_term (upRen_term_term xi_term) (up_term_term sigma_term)
+           (rinstInst_up_term_term _ _ Eq_term) s3)
   | app s0 s1 =>
       congr_app (rinst_inst_term xi_term sigma_term Eq_term s0)
         (rinst_inst_term xi_term sigma_term Eq_term s1)
@@ -980,10 +1004,11 @@ Fixpoint allfv_term (p_term : nat -> Prop) (s : term) {struct s} : Prop :=
               (and True
                  (and (allfv_term p_term s4)
                     (and (allfv_term (upAllfv_term_term p_term) s5) True)))))
-  | lam s0 s1 s2 =>
+  | lam s0 s1 s2 s3 =>
       and True
         (and (allfv_term p_term s1)
-           (and (allfv_term (upAllfv_term_term p_term) s2) True))
+           (and (allfv_term (upAllfv_term_term p_term) s2)
+              (and (allfv_term (upAllfv_term_term p_term) s3) True)))
   | app s0 s1 => and (allfv_term p_term s0) (and (allfv_term p_term s1) True)
   | Erased s0 => and (allfv_term p_term s0) True
   | erase s0 => and (allfv_term p_term s0) True
@@ -1028,12 +1053,15 @@ Fixpoint allfvTriv_term (p_term : nat -> Prop) (H_term : forall x, p_term x)
                     (conj
                        (allfvTriv_term (upAllfv_term_term p_term)
                           (upAllfvTriv_term_term H_term) s5) I)))))
-  | lam s0 s1 s2 =>
+  | lam s0 s1 s2 s3 =>
       conj I
         (conj (allfvTriv_term p_term H_term s1)
            (conj
               (allfvTriv_term (upAllfv_term_term p_term)
-                 (upAllfvTriv_term_term H_term) s2) I))
+                 (upAllfvTriv_term_term H_term) s2)
+              (conj
+                 (allfvTriv_term (upAllfv_term_term p_term)
+                    (upAllfvTriv_term_term H_term) s3) I)))
   | app s0 s1 =>
       conj (allfvTriv_term p_term H_term s0)
         (conj (allfvTriv_term p_term H_term s1) I)
@@ -1125,7 +1153,7 @@ allfv_term p_term s -> allfv_term q_term s :=
                                   end
                               end
                           end) I)))))
-  | lam s0 s1 s2 =>
+  | lam s0 s1 s2 s3 =>
       fun HP =>
       conj I
         (conj
@@ -1145,7 +1173,23 @@ allfv_term p_term s -> allfv_term q_term s :=
                                     | conj HP _ => HP
                                     end
                      end
-                 end) I))
+                 end)
+              (conj
+                 (allfvImpl_term (upAllfv_term_term p_term)
+                    (upAllfv_term_term q_term) (upAllfvImpl_term_term H_term)
+                    s3
+                    match HP with
+                    | conj _ HP =>
+                        match HP with
+                        | conj _ HP =>
+                            match HP with
+                            | conj _ HP =>
+                                match HP with
+                                | conj HP _ => HP
+                                end
+                            end
+                        end
+                    end) I)))
   | app s0 s1 =>
       fun HP =>
       conj
@@ -1361,7 +1405,7 @@ allfv_term (funcomp p_term xi_term) s :=
                                      end
                                  end
                              end)) I)))))
-  | lam s0 s1 s2 =>
+  | lam s0 s1 s2 s3 =>
       fun H =>
       conj I
         (conj
@@ -1382,7 +1426,23 @@ allfv_term (funcomp p_term xi_term) s :=
                                       | conj H _ => H
                                       end
                         end
-                    end)) I))
+                    end))
+              (conj
+                 (allfvImpl_term _ _ (upAllfvRenL_term_term p_term xi_term)
+                    s3
+                    (allfvRenL_term (upAllfv_term_term p_term)
+                       (upRen_term_term xi_term) s3
+                       match H with
+                       | conj _ H =>
+                           match H with
+                           | conj _ H =>
+                               match H with
+                               | conj _ H => match H with
+                                             | conj H _ => H
+                                             end
+                               end
+                           end
+                       end)) I)))
   | app s0 s1 =>
       fun H =>
       conj
@@ -1590,7 +1650,7 @@ allfv_term p_term (ren_term xi_term s) :=
                                      end
                                  end
                              end)) I)))))
-  | lam s0 s1 s2 =>
+  | lam s0 s1 s2 s3 =>
       fun H =>
       conj I
         (conj
@@ -1612,7 +1672,23 @@ allfv_term p_term (ren_term xi_term s) :=
                                       | conj H _ => H
                                       end
                         end
-                    end)) I))
+                    end))
+              (conj
+                 (allfvRenR_term (upAllfv_term_term p_term)
+                    (upRen_term_term xi_term) s3
+                    (allfvImpl_term _ _
+                       (upAllfvRenR_term_term p_term xi_term) s3
+                       match H with
+                       | conj _ H =>
+                           match H with
+                           | conj _ H =>
+                               match H with
+                               | conj _ H => match H with
+                                             | conj H _ => H
+                                             end
+                               end
+                           end
+                       end)) I)))
   | app s0 s1 =>
       fun H =>
       conj
